Rules for [deep_handler_body].

coq-osiris/theories/program_logic/handler_rules.v
@@ -142,13 +142,15 @@ Section handler_proof.
     by iApply (ewp_handle with "He").
   Qed.
 
-  Definition deep_handler_body η o bs := pre_eval_match_aux eval true η o bs bs.
+  Definition deep_handler_body := pre_eval_match_aux eval true.
+
+  Definition shallow_handler_body := pre_eval_match_aux eval false.
 
   (* Specification of [deep_handler] at the [expr] level. *)
   Lemma ewp_deep_handler E Ψ Φ Ψ' Φ' η e bs:
     EWP (eval η e) @ E <| Ψ |> {{ Φ }} -∗
     (* The deep handler specification is met *)
-    deep_handler_spec E Ψ Φ (λ o, deep_handler_body η o bs) Ψ' Φ' -∗
+    deep_handler_spec E Ψ Φ (λ o, deep_handler_body η o bs bs) Ψ' Φ' -∗
     EWP (deep_handler η e bs) @ E <| Ψ' |> {{ Φ' }}.
   Proof.
     (* We abstract away [eval η e]. *)
@@ -194,7 +196,7 @@ Section handler_proof.
         << λ o : outcome2 val exn, (* We need the annotation here; LATER: remove? *)
             ∀ Ψ'' Φ'',
               ▷ deep_handler_spec_def E Ψ Φ
-                (λ o, deep_handler_body η o bs) Ψ'' Φ'' -∗
+                (λ o, deep_handler_body η o bs bs) Ψ'' Φ'' -∗
               EWP stop CResume (l', o) @ E <| Ψ'' |> {{ Φ'' }} >>)%I
         with "[HP Hl]" as "HΨ".
       { iApply (monotonic_prot with "[Hl] HP"); iFrame.
@@ -205,7 +207,7 @@ Section handler_proof.
 
         (* Resume the continuation that stored the installed handler *)
         iApply (ewp_resume with "Hl"). iNext.
-        iIntros (?) "Hl". cbn.
+        iIntros "Hl". cbn.
         iSpecialize ("IH" with "H").
 
         (* Rewriting under binders for handle.. LATER: Remove? *)
@@ -226,5 +228,67 @@ Section handler_proof.
       rewrite deep_handler_spec_unfold.
       iApply ("IH" with "Hsh"). }
   Qed.
+
+  Lemma deep_handle_nil_ret η v all_branches ψ Φ :
+   EWP match_failure () <|ψ|> {{ Φ }} -∗
+   EWP (deep_handler_body η (O3Ret v) [] all_branches) <|ψ|> {{ Φ }}.
+  Proof.
+    by iIntros.
+  Qed.
+
+  Lemma deep_handle_nil_throw η e all_branches ψ Φ :
+   EWP throw e <|ψ|> {{ Φ }} -∗
+   EWP (deep_handler_body η (O3Throw e) [] all_branches) <|ψ|> {{ Φ }}.
+  Proof.
+    by iIntros.
+  Qed.
+
+  Lemma deep_handle_nil_perform η eff k all_branches ψ sk Φ :
+    k ↦ K sk -∗
+    ψ allows perform eff
+    << λ o,
+      ▷ (k ↦ Shot -∗ EWP (sk o) <|ψ|> {{ Φ }}) >> -∗
+    EWP (deep_handler_body η (O3Perform eff k) [] all_branches) <|ψ|> {{ Φ }}.
+  Proof.
+    iIntros "Hl Hperf".
+    iApply ewp_stop_perform.
+    rewrite /prot /iEff_car.
+    iApply (monotonic_prot (Ψ:=upcl OS ψ) with "[Hl]").
+    { iIntros (o) "H".
+      iPoseProof (ewp_resume with "Hl") as "Hcov".
+      iModIntro.
+      iApply "Hcov". rewrite try2_ret_right. iApply "H". }
+    done.
+  Qed.
+
+  Lemma deep_handle_cons deep η o cp e bs all_branches ψ Φ φ Q :
+    cpattern η cp o (λ δ, Q ⊢ EWP (eval δ e) <|ψ|> {{ Φ }}) φ ->
+    Q -∗
+    (⌜φ⌝ -∗ EWP (pre_eval_match_aux eval deep η o bs all_branches) <|ψ|> {{ Φ }}) -∗
+    EWP (pre_eval_match_aux eval deep η o (Branch cp e :: bs) all_branches) <|ψ|> {{ Φ }}.
+  Proof.
+    unfold cpattern.
+    iIntros (Hpat) "Q Hcov".
+    destruct Hpat as [ (δ & Hsimp & Hewp) | (exc & Hsimp & Hφ) ];
+      simpl; iApply ewp_try;
+      (iApply ewp_simp; [ eassumption | ]).
+    - iApply ewp_value; simpl. iApply (Hewp with "Q").
+    - iApply ewp_throw; simpl. iApply ("Hcov" $! Hφ).
+  Qed.
+
+  Lemma shallow_handle_cons η o cp e bs all_branches ψ Φ φ :
+    cpattern η cp o (λ δ, ⊢ EWP (eval δ e) <|ψ|> {{ Φ }}) φ ->
+    (⌜φ⌝ -∗ EWP (shallow_handler_body η o bs all_branches) <|ψ|> {{ Φ }}) -∗
+    EWP (shallow_handler_body η o (Branch cp e :: bs) all_branches) <|ψ|> {{ Φ }}.
+  Proof.
+    unfold cpattern, shallow_handler_body.
+    iIntros (Hpat) "Hcov".
+    destruct Hpat as [ (δ & Hsimp & Hewp) | (exc & Hsimp & Hφ) ];
+      simpl; iApply ewp_try;
+      (iApply ewp_simp; [ eassumption | ]).
+    - by iApply ewp_value.
+    - iApply ewp_throw; simpl. iApply ("Hcov" $! Hφ).
+  Qed.
+
 
 End handler_proof.
